Added tautology and contraction, but no examples to check with yet

src/trace/coqTerms.ml
@@ -281,6 +281,7 @@ let make_certif_ops modules args =
  (gen_constant "step",
   gen_constant "Res", gen_constant "Weaken", gen_constant "ImmFlatten",
   gen_constant "CTrue", gen_constant "CFalse", gen_constant "NotNot",
+  gen_constant "Tautology", gen_constant "Contraction",
   gen_constant "BuildDef", gen_constant "BuildDef2",
   gen_constant "BuildProj",
   gen_constant "ImmBuildProj", gen_constant"ImmBuildDef",
