src/trace/smtCertif.mli
@@ -30,6 +30,13 @@ type 'hform rule =
   | NotNot of 'hform
      (*  * notnot           : {(not not x) --> x}
      *)
+  | Tautology of 'hform clause * 'hform
+     (*  * tautology        : {(x_1 ... x_i ... (not x_i) ... x_n) --> true)}
+     *)
+  | Contraction of 'hform clause * 'hform list
+     (*  * contraction      : {(x_1 ... x_n) --> (x_k1 ... x_kn)}, 
+          where duplicates are removed and order is preserved 
+     *)
   | BuildDef of 'hform (* the first literal of the clause *)
      (*  * and_neg          : {(and a_1 ... a_n) (not a_1) ... (not a_n)}
          * or_pos           : {(not (or a_1 ... a_n)) a_1 ... a_n}
